Make cache purely thread-local
The cache now has no memory state, buffering purely in a state monad
with a cache (and no write buffer). Writes and proper cache misses (ie,
those that fill the cache) still require a write lock to protect the
disk. Non-filling reads are safe for any disk, whereas other operations
require that the cache rep apply to the physical disk, which can be
guaranteed with a write lock and by starting from a known good cache
(eg, by reading from memory and using the invariant).

Without a write buffer, there is no need for CacheCommit and CacheAbort
- higher levels will have to worry about writing the cache to memory,
and can abort by reverting to an earlier cache and its corresponding vd.

src/OptimisticCache.v
@@ -5,20 +5,13 @@ Require Import MemCache.
 Require Import FunctionalExtensionality.
 Require Import UpdList.
 
-(* re-export WriteBuffer since it's part of external type signatures *)
-Require Export WriteBuffer.
-
 Require SepAuto.
 
 Definition Disk := @mem addr addr_eq_dec valu.
 
-Record CacheParams :=
-  { cache : ident;
-    vdisk_committed : ident; }.
-
 Section OptimisticCache.
 
-  Implicit Types (c:Cache) (wb:WriteBuffer).
+  Implicit Types (c:Cache).
 
   Definition cache_rep (d: DISK) c (vd0: Disk) :=
     forall a, match cache_get c a with
@@ -33,55 +26,12 @@ Section OptimisticCache.
                      end
          end.
 
-  Definition wb_rep (vd0: Disk) wb (vd: Disk) :=
-    forall a, match wb_get wb a with
-         | Written v => vd a = Some v /\
-                       exists v0, vd0 a = Some v0
-         | WbMissing => vd a = vd0 a
-         end.
-
-  Definition no_pending_dirty (c: Cache) (wb: WriteBuffer) :=
-    forall a, cache_get c a = Invalid ->
-         wb_get wb a = WbMissing.
-
-  Variable (P:CacheParams).
   (* the protocol is completely arbitrary for the cache, since it never deals
   with locking *)
   Variable G:Protocol.
 
-  Definition CacheRep d wb (vd0 vd:Disk) : heappred :=
-    (exists c, cache P |-> val c *
-          (* why is AEQ required? seems like an inference bug *)
-          vdisk_committed P |-> absMem (AEQ:=addr_eq_dec) vd0 *
-          [[ cache_rep d c vd0 ]] *
-          [[ wb_rep vd0 wb vd ]] *
-          [[ no_pending_dirty c wb ]]
-    )%pred.
-
-  Lemma CacheRep_unfold : forall F m d wb vd0 vd,
-      (F * CacheRep d wb vd0 vd)%pred m ->
-      wb_rep vd0 wb vd /\
-      exists c, (F * cache P |-> val c * vdisk_committed P |-> absMem (AEQ:=addr_eq_dec) vd0)%pred m /\
-           cache_rep d c vd0 /\
-           no_pending_dirty c wb.
-  Proof.
-    unfold CacheRep; intros.
-    SepAuto.destruct_lifts; auto.
-    intuition.
-    eexists; intuition eauto.
-  Qed.
-
-  Lemma CacheRep_fold : forall F m d wb vd0 vd c,
-      (F * cache P |-> val c *
-       vdisk_committed P |-> absMem vd0)%pred m ->
-      cache_rep d c vd0 ->
-      wb_rep vd0 wb vd ->
-      no_pending_dirty c wb ->
-      (F * CacheRep d wb vd0 vd)%pred m.
-  Proof.
-    unfold CacheRep; intros.
-    SepAuto.pred_apply; SepAuto.cancel.
-  Qed.
+  Definition CacheRep d c (vd:Disk) :=
+    cache_rep d c vd.
 
   Ltac simplify :=
     repeat match goal with
@@ -90,9 +40,9 @@ Section OptimisticCache.
              let m := fresh m in
              destruct a as [m n]
            | [ |- exists (_: _ * _), _ ] => apply exists_tuple
+           | [ H: (_, _) = (_, _) |- _ ] =>
+             inversion H; subst; clear H
            | [ H: exists _, _ |- _ ] => deex
-           | [ H: (_ * CacheRep _ _ _ _)%pred _ |- _ ] =>
-             apply CacheRep_unfold in H; safe_intuition; deex
            | _ => progress simpl in *
            | _ => progress subst
            | _ => progress simpl_match
@@ -103,9 +53,6 @@ Section OptimisticCache.
   Ltac finisher :=
     descend;
     repeat match goal with
-           | [ |- cprog_ok _ _ _ _ ] => fail
-           | [ |- (_ * CacheRep _ _ _ _)%pred _ ] =>
-             eapply CacheRep_fold
            | [ |- ?F (Sigma.mem _) ] =>
              solve [ SepAuto.pred_apply; SepAuto.cancel ]
            | _ => congruence
@@ -116,525 +63,178 @@ Section OptimisticCache.
 
   Ltac step := CCLAutomation.step; simplify; finisher.
 
-  Definition BufferRead wb a :=
-    match wb_get wb a with
-    | Written v => Ret (Some v)
-    | WbMissing => Ret (None)
-    end.
-
-  Definition ClearPending c wb a :=
+  Definition ClearPending c a :=
     v <- WaitForRead a;
       let c' := add_entry Clean c a v in
-      _ <- Assgn (cache P) c';
-        (* note that v could also be added to the local write buffer (not
-           returned since it isn't modified), which should improve
-           performance *)
-        Ret v.
+        Ret (v, c').
 
-  Definition CacheRead wb a l :=
-    r <- BufferRead wb a;
-      match r with
-      | Some v => Ret (Some v, wb)
-      | None => c <- Get _ (cache P);
-                 match cache_get c a with
-                 | Present v _ => Ret (Some v, wb)
-                 | Missing => if CanWrite l then
-                               _ <- BeginRead a;
-                               let c' := mark_pending c a in
-                               _ <- Assgn (cache P) c';
-                                 Ret (None, wb)
-                             else Ret (None, wb)
-                 | Invalid => if CanWrite l then
-                               v <- ClearPending c wb a;
-                                 Ret (Some v, wb)
-                             else Ret (None, wb)
-                 end
-      end.
+  Definition CacheRead_nofill c a :=
+    match cache_get c a with
+    | Present v _ => Ret (Some v, c)
+    | Missing => Ret (None, c)
+    | Invalid => Ret (None, c)
+    end.
+
+  Definition CacheRead_fill c a :=
+    match cache_get c a with
+    | Present v _ => Ret (Some v, c)
+    | Missing => _ <- BeginRead a;
+                  let c' := mark_pending c a in
+                  Ret (None, c')
+    | Invalid => do '(v,c) <- ClearPending c a;
+                  Ret (Some v, c)
+    end.
 
   Ltac solve_cache :=
     unfold CacheRep; intuition;
     repeat match goal with
            | [ a: addr, H: cache_rep _ _ _ |- _ ] =>
              specialize (H a)
-           | [ a: addr, H: wb_rep _ _ _ |- _ ] =>
-             specialize (H a)
-           | [ a: addr, H: no_pending_dirty _ _ |- _ ] =>
-             specialize (H a)
            end;
     repeat simpl_match;
     repeat deex;
     intuition eauto; try congruence.
 
-  Lemma Buffer_hit:
-    forall (wb : WriteBuffer) (a : addr) (v : valu),
-      wb_get wb a = Written v ->
-      forall (vd0 vd : Disk) (v0 : valu), wb_rep vd0 wb vd -> vd a = Some v0 -> v = v0.
-  Proof.
-    solve_cache.
-  Qed.
-
-  Hint Resolve Buffer_hit.
-
-  Definition BufferRead_ok : forall tid wb a,
-      cprog_spec G tid
-                 (fun '(F, vd0, vd, v0) '(sigma_i, sigma) =>
-                    {| precondition :=
-                         (F * CacheRep (Sigma.disk sigma) wb vd0 vd)%pred (Sigma.mem sigma) /\
-                         vd a = Some v0;
-                       postcondition :=
-                         fun '(sigma_i', sigma') r =>
-                           sigma' = sigma /\
-                           match r with
-                           | Some v => v = v0
-                           | None => wb_get wb a = WbMissing
-                           end /\
-                           sigma_i' = sigma_i|})
-                 (BufferRead wb a).
-  Proof.
-    unfold BufferRead; intros.
-
-    case_eq (wb_get wb a); intros.
-    hoare finish.
-    hoare finish.
-  Qed.
-
-  Hint Extern 0 {{ BufferRead _ _; _ }} => apply BufferRead_ok : prog.
+  Hint Extern 3 (_ = _) => congruence.
 
   Lemma CacheRep_invalid:
-    forall (c : Cache) (wb : WriteBuffer) (a : addr) d (vd0 vd : Disk) (v0 : valu),
-      cache_rep d c vd0 ->
-      wb_rep vd0 wb vd ->
-      no_pending_dirty c wb ->
-      cache_get c a = Invalid -> vd a = Some v0 -> d a = Some (v0, Pending).
+    forall (c : Cache) (a : addr) d (vd : Disk) (v0 : valu),
+      CacheRep d c vd ->
+      cache_get c a = Invalid ->
+      vd a = Some v0 -> d a = Some (v0, Pending).
   Proof.
-    intros.
-    destruct (wb_get wb a) eqn:?;
-             solve_cache.
+    solve_cache.
   Qed.
 
   Hint Resolve CacheRep_invalid.
 
-  Lemma cache_rep_add_clean:
-    forall (c : Cache) (wb : WriteBuffer) (a : addr) (vd0 vd : Disk)
-      (v0 : valu) (d : DISK),
-      cache_rep d c vd0 ->
-      wb_rep vd0 wb vd ->
-      no_pending_dirty c wb ->
+  Lemma CacheRep_finish_read:
+    forall (c : Cache) (a : addr) d d' (vd : Disk) (v0 : valu),
+      CacheRep d c vd ->
       vd a = Some v0 ->
       cache_get c a = Invalid ->
-      forall d' : DISK,
-        d' = upd d a (v0, NoReader) -> cache_rep d' (add_entry Clean c a v0) vd0.
+      d' = upd d a (v0, NoReader) ->
+      CacheRep d' (add_entry Clean c a v0) vd.
   Proof.
-    intros.
-    unfold cache_rep; intros a'.
-    repeat match goal with
-           | [ H: _ |- _ ] =>
-             specialize (H a')
-           end.
-    destruct (addr_eq_dec a a'); simplify.
-    congruence.
-  Qed.
-
-  Lemma no_pending_dirty_add_clean:
-    forall (c : Cache) (wb : WriteBuffer) (a : addr) (v0 : valu),
-      no_pending_dirty c wb -> no_pending_dirty (add_entry Clean c a v0) wb.
-  Proof.
-    unfold no_pending_dirty; intros.
+    unfold CacheRep, cache_rep; intros.
     specialize (H a0).
-    destruct (addr_eq_dec a a0); simplify.
-    congruence.
+    destruct (addr_eq_dec a a0); subst;
+      autorewrite with cache upd;
+      solve_cache.
   Qed.
 
-  Hint Resolve cache_rep_add_clean no_pending_dirty_add_clean.
+  Hint Resolve CacheRep_finish_read.
 
-  Hint Extern 3 (_ = _) => congruence.
-
-  Theorem ClearPending_ok : forall tid c wb a,
+  Theorem ClearPending_ok : forall tid c a,
       cprog_spec G tid
-                 (fun '(F, vd0, vd, v0) '(sigma_i, sigma) =>
+                 (fun '(F, vd, v0) sigma =>
                     {| precondition :=
-                         (F * cache P |-> val c *
-                          vdisk_committed P |-> absMem vd0)%pred (Sigma.mem sigma) /\
-                         cache_rep (Sigma.disk sigma) c vd0 /\
-                         wb_rep vd0 wb vd /\
-                         no_pending_dirty c wb /\
+                         F (Sigma.mem sigma) /\
+                         CacheRep (Sigma.disk sigma) c vd /\
                          cache_get c a = Invalid /\
                          vd a = Some v0 /\
                          Sigma.l sigma = WriteLock;
                        postcondition :=
-                         fun '(sigma_i', sigma') r =>
-                           (exists c',
-                               (F * cache P |-> val c' *
-                                vdisk_committed P |-> absMem vd0)%pred (Sigma.mem sigma') /\
-                               cache_rep (Sigma.disk sigma') c' vd0 /\
-                               wb_rep vd0 wb vd /\
-                               no_pending_dirty c' wb /\
-                               cache_get c' a = Present v0 Clean) /\
+                         fun sigma' '(r, c') =>
+                           F (Sigma.mem sigma') /\
+                           CacheRep (Sigma.disk sigma') c' vd /\
+                           cache_get c' a = Present v0 Clean /\
                            r = v0 /\
                            Sigma.hm sigma' = Sigma.hm sigma /\
-                           sigma_i' = sigma_i /\
                            Sigma.l sigma' = Sigma.l sigma; |})
-                 (ClearPending c wb a).
+                 (ClearPending c a).
   Proof.
     unfold ClearPending.
     hoare finish.
-    finish.
-    simplify.
   Qed.
 
-  Hint Extern 0 {{ ClearPending _ _ _; _ }} => apply ClearPending_ok : prog.
+  Hint Extern 0 {{ ClearPending _ _; _ }} => apply ClearPending_ok : prog.
 
-  Lemma Buffer_miss_cache_hit:
-    forall (wb : WriteBuffer) (a : addr) d
-      (vd0 vd : Disk) (v0 : valu),
-      wb_rep vd0 wb vd ->
-      vd a = Some v0 ->
-      forall c : Cache,
-        cache_rep d c vd0 ->
-        wb_get wb a = WbMissing ->
-        forall (v : valu) (b : DirtyBit), cache_get c a = Present v b -> v = v0.
+  Lemma CacheRep_present_val:
+    forall (c : Cache) (a : addr) (v : valu) (b : DirtyBit),
+      cache_get c a = Present v b ->
+      forall (d : DISK) (vd : Disk) (v0 : valu),
+        CacheRep d c vd -> vd a = Some v0 -> v = v0.
   Proof.
     solve_cache.
   Qed.
 
-  Hint Resolve Buffer_miss_cache_hit.
+  Hint Resolve CacheRep_present_val.
 
-  Lemma CacheRep_missing:
-    forall (wb : WriteBuffer) (a : addr) (vd0 vd : Disk) (v0 : valu),
-      wb_rep vd0 wb vd ->
-      vd a = Some v0 ->
-      forall (c : Cache) (d : DISK),
-        cache_rep d c vd0 ->
-        wb_get wb a = WbMissing -> cache_get c a = Missing -> d a = Some (v0, NoReader).
-  Proof.
-    solve_cache.
-    rewrite H in *.
-    simpl_match; auto.
-  Qed.
-
-  Hint Resolve CacheRep_missing.
-
-  Lemma CacheRep_mark_pending:
-    forall (a : addr) (vd0 vd : Disk) (v0 : valu) (c : Cache) wb,
-      vd a = Some v0 ->
-      wb_rep vd0 wb vd ->
-      forall d : DISK,
-        cache_rep d c vd0 ->
-        cache_get c a = Missing ->
-        wb_get wb a = WbMissing ->
-        forall d' : DISK,
-          d' = upd d a (v0, Pending) -> cache_rep d' (mark_pending c a) vd0.
-  Proof.
-    unfold cache_rep; intros; subst.
-    repeat match goal with
-           | [ H: _ |- _ ] =>
-             specialize (H a0)
-           end.
-    destruct (addr_eq_dec a a0); simplify.
-  Qed.
-
-  Hint Resolve CacheRep_mark_pending.
-
-  Lemma no_pending_dirty_add_pending:
-    forall (wb : WriteBuffer) (a : addr) (c : Cache),
-      no_pending_dirty c wb ->
-      wb_get wb a = WbMissing -> no_pending_dirty (mark_pending c a) wb.
-  Proof.
-    unfold no_pending_dirty; intros.
-    destruct (addr_eq_dec a a0); simplify.
-  Qed.
-
-  Hint Resolve no_pending_dirty_add_pending.
-
-  Definition CacheRead_ok : forall tid wb a l,
+  Definition CacheRead_nofill_ok : forall tid c a,
       cprog_spec G tid
-                 (fun '(F, vd0, vd, v0) '(sigma_i, sigma) =>
+                 (fun '(F, d, vd, v0) sigma =>
                     {| precondition :=
-                         (F * CacheRep (Sigma.disk sigma) wb vd0 vd)%pred (Sigma.mem sigma) /\
-                         vd a = Some v0 /\
-                         Sigma.l sigma = l /\
-                         ReadPermission l;
+                         F (Sigma.mem sigma) /\
+                         CacheRep d c vd /\
+                         vd a = Some v0;
                        postcondition :=
-                         fun '(sigma_i', sigma') '(r, wb') =>
-                           (F * CacheRep (Sigma.disk sigma') wb' vd0 vd)%pred (Sigma.mem sigma') /\
-                           wb' = wb /\
+                         fun sigma' '(r, c') =>
+                           F (Sigma.mem sigma) /\
+                           CacheRep d c' vd /\
+                           c' = c /\
                            Sigma.hm sigma' = Sigma.hm sigma /\
                            match r with
                            | Some v => v = v0
                            | None => True
                            end /\
-                           sigma_i' = sigma_i /\
                            Sigma.l sigma' = Sigma.l sigma |})
-                 (CacheRead wb a l).
+                 (CacheRead_nofill c a).
   Proof.
-    unfold CacheRead.
-    hoare finish.
-
-    destruct r; hoare finish.
-
-    rename r into c'.
-    destruct (cache_get c' a) eqn:?; hoare finish.
-    destruct (CanWrite (Sigma.l sigma)); hoare finish.
-    destruct (CanWrite (Sigma.l sigma)); hoare finish.
+    unfold CacheRead_nofill.
+    intros.
+    destruct (cache_get c a) eqn:?; hoare finish.
   Qed.
 
-  Definition CacheWrite wb a v :=
-    c <- Get _ (cache P);
-      _ <- match cache_get c a with
-          | Invalid => _ <- ClearPending c wb a;
-                        Ret tt
-          | _ => Ret tt
-          end;
-      Ret (tt, wb_add wb a v).
+  Definition CacheWrite c a v :=
+    c <- match cache_get c a with
+        | Invalid => do '(_, c) <- ClearPending c a;
+                      Ret c
+        | _ => Ret c
+        end;
+      let c' := add_entry Dirty c a v in
+      Ret (tt, c').
 
-  Lemma wb_rep_add:
-    forall (wb : WriteBuffer) (a : addr) (v : valu) (vd0 vd : Disk) (v0 : valu),
-      wb_rep vd0 wb vd ->
-      forall c : Cache, vd a = Some v0 ->
-                   no_pending_dirty c wb ->
-                   cache_get c a <> Invalid ->
-                   wb_rep vd0 (wb_add wb a v) (upd vd a v).
-  Proof.
-    unfold wb_rep; intros.
-    repeat match goal with
-           | [ H: _ |- _ ] =>
-             specialize (H a0)
-           end.
-    destruct (addr_eq_dec a a0); simplify.
-    destruct (wb_get wb a0) eqn:?; simplify.
-    rewrite <- H; eauto.
-  Qed.
-
-  Hint Resolve wb_rep_add.
-
-  Lemma no_pending_dirty_add:
-    forall (wb : WriteBuffer) (a : addr) (v : valu) (c : Cache),
-      no_pending_dirty c wb ->
+  Lemma CacheRep_dirty_write:
+    forall (c : Cache) (a : addr) (v : valu),
       cache_get c a <> Invalid ->
-      no_pending_dirty c (wb_add wb a v).
+      forall (vd : Disk) (v1 : valu) d,
+        CacheRep d c vd ->
+        vd a = Some v1 ->
+        CacheRep d (add_entry Dirty c a v) (upd vd a v).
   Proof.
-    unfold no_pending_dirty; intros.
-    specialize (H a0).
-    destruct (addr_eq_dec a a0); simplify.
+    unfold CacheRep, cache_rep; intros.
+    specialize (H0 a0).
+    destruct (addr_eq_dec a a0); subst;
+      autorewrite with cache upd;
+      solve_cache.
+    destruct (cache_get c a0) eqn:Hcache;
+      intuition eauto.
+    destruct b; eauto.
   Qed.
 
-  Hint Resolve no_pending_dirty_add.
-
+  Hint Resolve CacheRep_dirty_write.
   Hint Extern 2 (cache_get _ _ <> _) => congruence.
 
-  Theorem CacheWrite_ok : forall tid wb a v,
+  Theorem CacheWrite_ok : forall tid c a v,
       cprog_spec G tid
-                 (fun '(F, vd0, vd, v0) '(sigma_i, sigma) =>
+                 (fun '(F, vd, v0) sigma =>
                     {| precondition :=
-                         (F * CacheRep (Sigma.disk sigma) wb vd0 vd)%pred (Sigma.mem sigma) /\
+                         F (Sigma.mem sigma) /\
+                         CacheRep (Sigma.disk sigma) c vd /\
                          vd a = Some v0 /\
                          Sigma.l sigma = WriteLock;
                        postcondition :=
-                         fun '(sigma_i', sigma') '(_, wb') =>
-                           (F * CacheRep (Sigma.disk sigma') wb' vd0 (upd vd a v))%pred (Sigma.mem sigma') /\
+                         fun sigma' '(_, c') =>
+                           F (Sigma.mem sigma') /\
+                           CacheRep (Sigma.disk sigma') c' (upd vd a v) /\
                            Sigma.hm sigma' = Sigma.hm sigma /\
-                           Sigma.l sigma' = Sigma.l sigma /\
-                           sigma_i' = sigma_i; |})
-                 (CacheWrite wb a v).
+                           Sigma.l sigma' = Sigma.l sigma; |})
+                 (CacheWrite c a v).
   Proof.
     unfold CacheWrite.
-    hoare finish.
-    rename r into c'.
-    destruct (cache_get c' a) eqn:?; hoare finish.
-  Qed.
-
-  Fixpoint add_writes (c:Cache) (wrs: list (addr * valu)) :=
-    match wrs with
-    | nil => c
-    | (a,v) :: wrs' => add_entry Dirty (add_writes c wrs') a v
-    end.
-
-  Definition upd_with_buffer (c:Cache) (wb:WriteBuffer) :=
-    add_writes c (wb_writes wb).
-
-  Definition CacheCommit wb :=
-    c <- Get _ (cache P);
-      _ <- Assgn (cache P) (upd_with_buffer c wb);
-      _ <- GhostUpdateMem (vdisk_committed P) (fun _ (vd0:Disk) =>
-                                                upd_all vd0 (wb_writes wb));
-      Ret tt.
-
-  Lemma no_pending_dirty_empty : forall c,
-      no_pending_dirty c empty_writebuffer.
-  Proof.
-    unfold no_pending_dirty; eauto.
-  Qed.
-
-  Lemma wb_rep_empty : forall vd,
-      wb_rep vd empty_writebuffer vd.
-  Proof.
-    unfold wb_rep; intros; simpl; auto.
-  Qed.
-
-  Hint Resolve no_pending_dirty_empty wb_rep_empty.
-
-  Theorem wb_rep_upd_all_ext : forall wb vd0 (vd: Disk) (a: addr),
-      wb_rep vd0 wb vd ->
-      vd a = upd_all (AEQ:=addr_eq_dec) vd0 (wb_writes wb) a.
-  Proof.
-    intro.
-    assert (forall a v, wb_get wb a = Written v <-> List.In (a, v) (wb_writes wb)).
-    { intros; apply wb_get_writes. }
     intros.
-    specialize (H a).
-    pose proof (wb_writes_nodup_addr wb).
-    move H1 at top.
-    generalize dependent (wb_writes wb).
-    induction l; intros; subst; simpl in *.
-    - specialize (H0 a).
-      case_eq (wb_get wb a); intros; simpl_match; auto.
-      exfalso.
-      eapply H; eauto.
-    - destruct a0 as [a' v].
-      destruct (addr_eq_dec a a'); subst; autorewrite with upd.
-      + destruct (H v) as [H' ?]; clear H'.
-        intuition.
-        specialize (H0 a'); simpl_match; intuition.
-      + simpl in *.
-        inversion H1; subst; intuition.
-
-        case_eq (wb_get wb a); intuition.
-        specialize (H v0); intuition.
-        erewrite upd_all_nodup_in by eauto.
-        specialize (H0 a); simpl_match; intuition eauto.
-
-        destruct (list_addr_in_dec addr_eq_dec a l);
-          autorewrite with upd.
-        destruct s.
-        specialize (H x); intuition.
-        specialize (H0 a); simpl_match; eauto.
-  Qed.
-
-  Corollary wb_rep_upd_all : forall vd0 wb vd,
-      wb_rep vd0 wb vd ->
-      vd = upd_all vd0 (wb_writes wb).
-  Proof.
-    intros.
-    extensionality a.
-    apply wb_rep_upd_all_ext; auto.
-  Qed.
-
-  Lemma cache_rep_add_dirty:
-    forall (d : DISK) (a : addr) (v : valu) (c : Cache) (vd0 : Disk),
-      cache_get c a <> Invalid ->
-      (exists v0, vd0 a = Some v0) ->
-      cache_rep d c vd0 ->
-      cache_rep d (add_entry Dirty c a v) (upd vd0 a v).
-  Proof.
-    unfold cache_rep; intros; repeat deex.
-    specialize (H1 a0).
-    destruct (addr_eq_dec a a0); subst; simplify; intuition eauto.
-    case_eq (cache_get c a0); intros; simpl_match; intuition.
-    destruct b; repeat deex; intuition eauto.
-    eauto.
-  Qed.
-
-  Lemma add_writes_same_invalid : forall ws c a,
-      cache_get (add_writes c ws) a = Invalid ->
-      cache_get c a = Invalid.
-  Proof.
-    induction ws; intros; simpl in *; auto.
-    destruct a as [a v].
-    destruct (addr_eq_dec a a0); subst;
-      autorewrite with cache in H; auto.
-  Qed.
-
-  Hint Resolve upd_all_incr_domain.
-
-  Lemma wb_domain_committed : forall vd0 wb vd,
-      wb_rep vd0 wb vd ->
-      (forall a v, wb_get wb a = Written v ->
-              exists v0, vd0 a = Some v0).
-  Proof.
-    intros.
-    specialize (H a); simpl_match; intuition eauto.
-  Qed.
-
-  Lemma cache_rep_commit : forall vd0 c wb d,
-      cache_rep d c vd0 ->
-      (forall a v, wb_get wb a = Written v ->
-              exists v0, vd0 a = Some v0) ->
-      no_pending_dirty c wb ->
-      cache_rep d (upd_with_buffer c wb) (upd_all vd0 (wb_writes wb)).
-  Proof.
-    intros.
-    unfold upd_with_buffer.
-    assert (forall a v, List.In (a,v) (wb_writes wb) ->
-                   wb_get wb a = Written v).
-    intros; apply wb_get_writes; auto.
-    generalize dependent (wb_writes wb); intros.
-    induction l; simpl; eauto.
-    destruct a as [a v].
-    pose proof (H2 a v); simpl in *; intuition.
-
-    eapply cache_rep_add_dirty; eauto.
-    - intro Hinvalid.
-      apply add_writes_same_invalid in Hinvalid.
-      specialize (H1 a); intuition congruence.
-  Qed.
-
-  (* express [cache_rep_commit] in a more automation-friendly form *)
-  Lemma cache_rep_commit_CacheRep :
-    forall (wb : WriteBuffer) (vd0 vd : Disk) c d d',
-      cache_rep d c vd0 ->
-      wb_rep vd0 wb vd ->
-      no_pending_dirty c wb ->
-      d = d' ->
-      cache_rep d' (upd_with_buffer c wb) vd.
-  Proof.
-    intros; subst.
-    erewrite wb_rep_upd_all by eauto.
-    apply cache_rep_commit; auto.
-    eapply wb_domain_committed; eauto.
-  Qed.
-
-  Hint Resolve cache_rep_commit_CacheRep.
-
-  Definition CacheCommit_ok : forall tid wb,
-      cprog_spec G tid
-                 (fun '(F, vd0, vd) '(sigma_i, sigma) =>
-                    {| precondition :=
-                         (F * CacheRep (Sigma.disk sigma) wb vd0 vd)%pred (Sigma.mem sigma) /\
-                         Sigma.l sigma = WriteLock;
-                       postcondition :=
-                         fun '(sigma_i', sigma') _ =>
-                           (F * CacheRep (Sigma.disk sigma') empty_writebuffer vd vd)%pred (Sigma.mem sigma') /\
-                           Sigma.hm sigma' = Sigma.hm sigma /\
-                           Sigma.l sigma' = Sigma.l sigma /\
-                           sigma_i' = sigma_i |})
-                 (CacheCommit wb).
-  Proof.
-    unfold CacheCommit.
-    hoare finish.
-    finish.
-    SepAuto.pred_apply; SepAuto.cancel.
-    erewrite <- wb_rep_upd_all by eauto; auto.
-  Qed.
-
-  Definition CacheAbort :=
-    Ret tt.
-
-  Definition CacheAbort_ok : forall tid,
-      cprog_spec G tid
-                 (fun '(F, vd0, vd, wb) '(sigma_i, sigma) =>
-                    {| precondition :=
-                         (F * CacheRep (Sigma.disk sigma) wb vd0 vd)%pred (Sigma.mem sigma);
-                       postcondition :=
-                         fun '(sigma_i', sigma') _ =>
-                           (F * CacheRep (Sigma.disk sigma')
-                                         empty_writebuffer vd0 vd0)%pred (Sigma.mem sigma') /\
-                           Sigma.hm sigma' = Sigma.hm sigma /\
-                           Sigma.l sigma' = Sigma.l sigma /\
-                           sigma_i' = sigma_i |})
-                 (CacheAbort).
-  Proof.
-    unfold CacheAbort.
-    hoare finish.
+    destruct (cache_get c a) eqn:?; hoare finish; simplify.
   Qed.
 
 End OptimisticCache.
