src/CCLHoareTriples.v
@@ -114,18 +114,6 @@ Section HoareTriples.
 
 End HoareTriples.
 
-Ltac spec_monad_simpl :=
-  let rewrite_equiv H := eapply spec_respects_exec_equiv;
-                         [ solve [ apply H ] | ] in
-  repeat match goal with
-         | [ |- cprog_spec _ _ _ (Bind _ (Ret _)) ] =>
-           rewrite_equiv monad_right_id
-         | [ |- cprog_spec _ _ _ (Bind (Ret _) _) ] =>
-           rewrite_equiv monad_left_id
-         | [ |- cprog_spec _ _ _ (Bind (Bind _ _) _) ] =>
-           rewrite_equiv monad_assoc
-         end.
-
 (* Local Variables: *)
 (* company-coq-local-symbols: (("Sigma" . ?Σ) ("sigma" . ?σ) ("sigma'" . (?σ (Br . Bl) ?'))) *)
 (* End: *)
